new/proof/github_com/goose_lang/goose/model/channel/logatom/chan_au_base.v
@@ -391,7 +391,8 @@ Proof.
   by iApply (ghost_var_agree with "Hchanrepfrag1 Hchanrepfrag2").
 Qed.
 
-Lemma own_channel_halves_update ch s s' s'' γ :
+(* Needs [chan_cap_valid s'' cap] as precondition? *)
+Lemma own_channel_halves_update s'' ch s s' γ :
   chan_cap_valid s'' (chan_cap γ) →
   own_channel ch s γ -∗ own_channel ch s' γ ==∗
   own_channel ch s'' γ ∗ own_channel ch s'' γ.
@@ -468,7 +469,25 @@ Definition rcv_au_slow ch (γ: chan_names) (Φ : V → bool → iProp Σ) : iPro
     end).
 
 (** Fast path receive: immediate completion when possible *)
-Definition rcv_au_fast ch (γ: chan_names) (Φ : V → bool → iProp Σ) : iProp Σ :=
+Definition rcv_au_fast ch γ (Φ : V → bool → iProp Σ) Φnotready : iProp Σ :=
+  (|={⊤,∅}=>
+     ▷∃ s, "Hoc" ∷ own_channel ch s γ ∗
+           "Hcont" ∷
+             match s with
+             (* Case: Sender is waiting, can complete immediately *)
+             | chan_rep.SndPending v =>
+                 own_channel ch chan_rep.RcvCommit γ ={∅,⊤}=∗ Φ v true
+             (* Case: Channel is closed *)
+             | chan_rep.Closed [] => own_channel ch s γ ={∅,⊤}=∗ Φ (default_val V) false
+             (* Case: Channel is closed but still has values to drain *)
+             | chan_rep.Closed (v::rest) => (own_channel ch (chan_rep.Closed rest) γ ={∅,⊤}=∗ Φ v true)
+             (* Case: Buffered channel with values *)
+             | chan_rep.Buffered (v::rest) => (own_channel ch (chan_rep.Buffered rest) γ ={∅,⊤}=∗ Φ v true)
+             | _ => True
+             end) ∧
+  Φnotready.
+
+Definition rcv_au_fast_alt ch γ (Φ : V → bool → iProp Σ) Φnotready : iProp Σ :=
    |={⊤,∅}=>
     ▷∃ s, "Hoc" ∷ own_channel ch s γ ∗
      "Hcont" ∷
@@ -482,15 +501,15 @@ Definition rcv_au_fast ch (γ: chan_names) (Φ : V → bool → iProp Σ) : iPro
     | chan_rep.Closed (v::rest) => (own_channel ch (chan_rep.Closed rest) γ ={∅,⊤}=∗ Φ v true)
     (* Case: Buffered channel with values *)
     | chan_rep.Buffered (v::rest) => (own_channel ch (chan_rep.Buffered rest) γ ={∅,⊤}=∗ Φ v true)
-    | _ => True
+    | _ => (own_channel ch s γ ={∅,⊤}=∗ Φnotready)
     end).
 
-Lemma blocking_rcv_implies_nonblocking ch γ Φ :
+Lemma blocking_rcv_implies_nonblocking ch γ (Φ : V → bool → iProp Σ) :
   rcv_au_slow ch γ Φ -∗
-  rcv_au_fast ch γ Φ.
+  rcv_au_fast ch γ Φ True.
 Proof.
   iIntros "Hau".
-  iMod "Hau" as (s) "[Hoc Hcont]".
+  iSplitL; last done. iMod "Hau" as (s) "[Hoc Hcont]".
   iModIntro. iExists s. iFrame "Hoc".
   destruct s; try done.
 Qed.
@@ -533,29 +552,73 @@ Definition send_au_slow ch (v : V) (γ: chan_names) (Φ : iProp Σ) : iProp Σ :
     end).
 
 (** Fast path send: immediate completion when possible *)
-Definition send_au_fast ch (v : V) (γ: chan_names) (Φ : iProp Σ) : iProp Σ :=
-   |={⊤,∅}=>
+Definition send_au_fast ch (v : V) γ Φ Φnotready : iProp Σ :=
+  (|={⊤,∅}=>
+     ▷∃ s, "Hoc" ∷ own_channel ch s γ ∗
+           "Hcont" ∷
+             match s with
+             (* Case: Receiver is waiting, can complete immediately *)
+             | chan_rep.RcvPending =>
+                 own_channel ch (chan_rep.SndCommit v) γ ={∅,⊤}=∗ Φ
+             (* Case: Channel is closed, client must rule this out *)
+             | chan_rep.Closed draining => False
+             (* Case: Buffered channel *)
+             | chan_rep.Buffered buff =>
+                   (own_channel ch (chan_rep.Buffered (buff ++ [v])) γ ={∅,⊤}=∗ Φ)
+             | _ => True
+             end) ∧
+  Φnotready.
+
+(* Q: is there a good way to combine this and [send_au_fast]?
+   complexity? The (∃ b) stuff comes from writing out the join of the two
+   incomparable specs (the old one and the new one).
+
+   old spec := ((|={⊤,∅}=> T ∨ N) ∧ Ψ)
+   new spec := (|={⊤,∅}=> T ∨ (N ∗ (N ={∅,⊤}=∗ Ψ)))
+   where T := (R ∗ (D ={∅,⊤}=∗ Φ)), where N is ownership of a not-ready state, R
+   is ownership of a ready state, D is ownership of a done state, and Ψ =
+   Φnotready.
+
+   One can't prove (new_spec -∗ old_spec) because Ψ in new_spec gets to rely on
+   knowing it only runs in the notready case. Also
+
+   One also probably can't prove (old_spec -∗ new_spec) because (among other
+   possible reasons) old spec does not provide `|={∅,⊤}=>` in the notready case,
+   and we'd need to somehow close all invariants. This challenge of "I decided I
+   don't want to update any ghost state, so I'd like to close all invariants by
+   putting everything back as it was" has the feeling of aborting in logical
+   atomicity (though it does *not* require a fixpoint to reestablish the entire
+   update).
+
+   (old spec) ∨ (new spec) =
+   ((atomic update with only Φ) ∧ Φnotready) ∨ (atomic update update to either Φ or Φnotready) =
+   ∃ b,
+   (atomic update with Φ and (if (not b) then Φnotready is included)) ∧ (if b then Φnotready) *)
+Definition send_au_fast_alt ch (v : V) γ Φ Φnotready : iProp Σ :=
+  |={⊤,∅}=>
     ▷∃ s, "Hoc" ∷ own_channel ch s γ ∗
-     "Hcont" ∷
-    (match s with
-    (* Case: Receiver is waiting, can complete immediately *)
-    | chan_rep.RcvPending =>
-        own_channel ch (chan_rep.SndCommit v) γ ={∅,⊤}=∗ Φ
-    (* Case: Channel is closed, client must rule this out *)
-    | chan_rep.Closed draining => False
-    (* Case: Buffered channel *)
-    | chan_rep.Buffered buff =>
-        (* own_channel implies new buffer size is <= cap, so the whole update is
-        equivalent to True if no space is available *)
-        (own_channel ch (chan_rep.Buffered (buff ++ [v])) γ ={∅,⊤}=∗ Φ)
-    | _ => True
-    end).
+          "Hcont" ∷
+            match s with
+            (* Case: Receiver is waiting, can complete immediately *)
+            | chan_rep.RcvPending =>
+                own_channel ch (chan_rep.SndCommit v) γ ={∅,⊤}=∗ Φ
+            (* Case: Channel is closed, client must rule this out *)
+            | chan_rep.Closed draining => False
+            (* Case: Buffered channel *)
+            | chan_rep.Buffered buff =>
+                if decide (length buff < chan_cap γ) then
+                  (own_channel ch (chan_rep.Buffered (buff ++ [v])) γ ={∅,⊤}=∗ Φ)
+                else
+                  (own_channel ch s γ ={∅,⊤}=∗ Φnotready)
+            | _ => (own_channel ch s γ ={∅,⊤}=∗ Φnotready)
+            end.
 
 Lemma blocking_send_implies_nonblocking ch v γ (Φ : iProp Σ) :
   send_au_slow ch v γ Φ -∗
-  send_au_fast ch v γ Φ.
+  send_au_fast ch v γ Φ True.
 Proof.
   iIntros "Hchan".
+  iSplitL; last done.
   iMod "Hchan" as (s) "[Hoc Hcont]".
   iModIntro. iExists s. iFrame "Hoc".
   destruct s; try done.
