new/golang/theory/chan.v
@@ -87,6 +87,13 @@ Proof.
   by iApply "HΦ".
 Qed.
 
+End proof.
+
+Section select_proof.
+
+Context `{hG: heapGS Σ, !ffi_semantics _ _}.
+Context `{!globalsGS Σ} {go_ctx : GoContext}.
+
 Inductive op :=
 | select_send_f (t: go_type) (v : val) (ch : chan.t) (handler : func.t)
 | select_receive_f (t: go_type) (ch : chan.t) (handler : func.t).
@@ -100,20 +107,147 @@ Global Instance into_val_op : IntoVal op :=
         end
   |}.
 
-Global Instance wp_select_send ch (v : val) f :
+Global Instance wp_select_send `{!IntoVal V} `{!IntoValTyped V t} ch (v : val) f :
   PureWp True (chan.select_send #t #ch v #f)
     #(select_send_f t v ch f).
 Proof.
   pure_wp_start. repeat rewrite to_val_unseal /=. by iApply "HΦ".
 Qed.
 
-Global Instance wp_select_receive ch f :
+Global Instance wp_select_receive `{!IntoVal V} `{!IntoValTyped V t} ch f :
   PureWp True (chan.select_receive #t #ch #f)
     #(select_receive_f t ch f).
 Proof.
   pure_wp_start. repeat rewrite to_val_unseal /=. by iApply "HΦ".
 Qed.
 
+(* The lemmas use Ψ because the original client-provided `send/rcv_au_slow` will
+   have some specific postcondition predicate. We don't want to force the caller
+   to transform that into a `send_au_slow` of a different. So, these lemmas are
+   written to take a wand that turns Ψ into Φ. *)
+Local Lemma wp_try_select_case_blocking cs Ψ :
+  ∀ Φ,
+  (match cs with
+   | select_send_f t send_val send_chan send_handler =>
+       ∃ V γ (v : V) `(!IntoVal V) `(!chanG Σ V) `(!IntoValTyped V t),
+     ⌜ send_val = #v ⌝ ∗
+     is_channel (V:=V) (t:=t) send_chan γ ∗
+     send_au_slow send_chan v γ (WP #send_handler #() {{ Ψ }})
+  | select_receive_f t recv_chan recv_handler =>
+      ∃ V γ `(!IntoVal V) `(!IntoValTyped V t) `(!chanG Σ V),
+     is_channel (V:=V) (t:=t) recv_chan γ ∗
+     rcv_au_slow recv_chan γ (λ (v: V) ok,
+                                    WP #recv_handler (#v, #ok)%V {{ Ψ }})
+   end
+  ) ∧ (Φ (#(), #false)%V) -∗
+  (∀ retv, Ψ retv -∗ Φ (retv, #true)%V) -∗
+  WP chan.try_select_case #cs #true {{ Φ }}.
+Proof.
+  iIntros (Φ) "HΦ Hwand".
+  wp_call. rewrite [in (_ op)]to_val_unseal /=. destruct cs; wp_auto.
+  - repeat setoid_rewrite bi.and_exist_r.
+    iDestruct "HΦ" as (V γ v' ? ? ?) "HΦ".
+    iNamed "HΦ". iAssert (⌜ v = #v' ⌝ ∗ is_channel ch γ)%I with "[-]" as "[-> #?]".
+    { iLeft in "HΦ". iDestruct "HΦ" as "(-> & #? & Hau)". iFrame "#". done. }
+    wp_apply (wp_TrySend with "[$]").
+    iSplit.
+    + iLeft in "HΦ". iDestruct "HΦ" as "(_ & _ & Hau)".
+      iMod "Hau". iModIntro. iNext. iNamed "Hau".
+      iFrame. destruct s.
+      * iIntros "H". iSpecialize ("Hcont" with "[$]").
+        iMod "Hcont". iModIntro. wp_auto.
+        wp_apply (wp_wand with "Hcont").
+        iIntros (?) "HΦ". wp_auto. iApply "Hwand". iFrame.
+      * iIntros "H". iSpecialize ("Hcont" with "[$]"). iMod "Hcont". iModIntro.
+        iMod "Hcont". iModIntro. iNext. iNamed "Hcont". iFrame.
+        destruct s; try iFrame. iIntros "H". iSpecialize ("Hcontinner" with "[$]").
+        iMod "Hcontinner". iModIntro. wp_auto. wp_apply (wp_wand with "Hcontinner").
+        iIntros (v) "HΦ". wp_auto. iApply "Hwand". iFrame.
+      * iFrame.
+      * iIntros "H". iSpecialize ("Hcont" with "[$]"). iMod "Hcont". iModIntro.
+        wp_auto. wp_apply (wp_wand with "Hcont"). iIntros (v) "HΦ".
+        wp_auto. iApply "Hwand". iFrame.
+      * iFrame.
+      * iFrame.
+      * iFrame.
+    + wp_auto. iRight in "HΦ". done.
+  - repeat setoid_rewrite bi.and_exist_r.
+    iDestruct "HΦ" as (V γ ? ? ?) "HΦ".
+    iAssert (is_channel ch γ)%I with "[-]" as "#?".
+    { iLeft in "HΦ". iDestruct "HΦ" as "(#? & Hau)". iFrame "#". }
+    wp_apply (wp_TryReceive with "[$]").
+    iSplit.
+    + iLeft in "HΦ". iDestruct "HΦ" as "[_ Hau]".
+      iMod "Hau". iModIntro. iNext.
+      iNamed "Hau". iFrame. destruct s.
+      * destruct buff.
+        -- iFrame.
+        -- iIntros "H". iSpecialize ("Hcont" with "[$]").
+           iMod "Hcont". iModIntro. wp_auto.
+           wp_apply (wp_wand with "Hcont").
+           iIntros (?) "HΦ". wp_auto. iApply "Hwand". iFrame.
+      * iIntros "H". iSpecialize ("Hcont" with "[$]"). iMod "Hcont". iModIntro.
+        iMod "Hcont". iModIntro. iNext. iNamed "Hcont". iFrame.
+        destruct s; try iFrame.
+        -- iIntros "H". iSpecialize ("Hcontinner" with "[$]").
+           iMod "Hcontinner". iModIntro. wp_auto. wp_apply (wp_wand with "Hcontinner").
+           iIntros (ret) "HΦ". wp_auto. iApply "Hwand". iFrame.
+        -- destruct draining; try iFrame.
+           iIntros "H". iSpecialize ("Hcontinner" with "[$]").
+           iMod "Hcontinner". iModIntro. wp_auto. wp_apply (wp_wand with "Hcontinner").
+           iIntros (ret) "HΦ". wp_auto. iApply "Hwand". iFrame.
+      * iIntros "H". iSpecialize ("Hcont" with "[$]").
+        iMod "Hcont". iModIntro. wp_auto. wp_apply (wp_wand with "Hcont").
+        iIntros (ret) "HΦ". wp_auto. iApply "Hwand". iFrame.
+      * iFrame.
+      * iFrame.
+      * iFrame.
+      * destruct draining.
+        -- iIntros "H". iSpecialize ("Hcont" with "[$]").
+           iMod "Hcont". iModIntro. wp_auto. wp_apply (wp_wand with "Hcont").
+           iIntros (ret) "HΦ". wp_auto. iApply "Hwand". iFrame.
+        -- iIntros "H". iSpecialize ("Hcont" with "[$]").
+           iMod "Hcont". iModIntro. wp_auto. wp_apply (wp_wand with "Hcont").
+           iIntros (ret) "HΦ". wp_auto. iApply "Hwand". iFrame.
+    + wp_auto. iRight in "HΦ". iFrame.
+Qed.
+
+Local Lemma wp_try_select_blocking (cases : list op) :
+  ∀ Ψ Φ,
+  ([∧ list] case ∈ cases,
+     match case with
+     | select_send_f t send_val send_chan send_handler =>
+         ∃ V γ (v : V) `(!IntoVal V) `(!chanG Σ V) `(!IntoValTyped V t),
+     ⌜ send_val = #v ⌝ ∗
+     is_channel (V:=V) (t:=t) send_chan γ ∗
+     send_au_slow send_chan v γ (WP #send_handler #() {{ Ψ }})
+  | select_receive_f t recv_chan recv_handler =>
+      ∃ V γ `(!IntoVal V) `(!IntoValTyped V t) `(!chanG Σ V),
+     is_channel (V:=V) (t:=t) recv_chan γ ∗
+     rcv_au_slow recv_chan γ (λ (v: V) ok,
+                                    WP #recv_handler (#v, #ok)%V {{ Ψ }})
+   end
+  ) ∧ Φ (#(), #false)%V -∗
+  □(∀ retv, Ψ retv -∗ Φ (retv, #true)%V) -∗
+  WP chan.try_select #cases #true {{ Φ }}.
+Proof.
+  simpl. iIntros (Ψ Φ) "HΦ #Hwand".
+  iLöb as "IH" forall (cases).
+  wp_call.
+  destruct cases.
+  { wp_auto. iRight in "HΦ". iApply "HΦ". }
+  wp_auto.
+  wp_apply (wp_try_select_case_blocking _ Ψ with "[-Hwand] [Hwand]").
+  2:{ iIntros (?) "HΨ". wp_auto. iApply "Hwand". iFrame. }
+  iSplit.
+  { simpl. iLeft in "HΦ". iLeft in "HΦ". iFrame. }
+  wp_auto. wp_apply ("IH" with "[HΦ]"); try iFrame.
+  iSplit.
+  - iLeft in "HΦ". simpl. iRight in "HΦ". iFrame.
+  - iRight in "HΦ". done.
+Qed.
+
+(* FIXME: rename fast and slow. *)
 Lemma wp_select_blocking (cases : list op) :
   ∀ Φ,
   ([∧ list] case ∈ cases,
@@ -124,7 +258,7 @@ Lemma wp_select_blocking (cases : list op) :
              is_channel (V:=V) (t:=t) send_chan γ ∗
              send_au_slow send_chan v γ (WP #send_handler #() {{ Φ }})
      | select_receive_f t recv_chan recv_handler =>
-         ∃ γ V `(!IntoVal V) `(!IntoValTyped V t) `(!chanG Σ V),
+         ∃ V γ `(!IntoVal V) `(!IntoValTyped V t) `(!chanG Σ V),
              is_channel (V:=V) (t:=t) recv_chan γ ∗
              rcv_au_slow recv_chan γ (λ (v: V) ok,
                WP #recv_handler (#v, #ok)%V {{ Φ }})
@@ -133,9 +267,119 @@ Lemma wp_select_blocking (cases : list op) :
   WP chan.select_blocking #cases {{ Φ }}.
 Proof.
   iIntros (Φ) "Hcases".
-  iLöb as "IH".
+  iLöb as "IH" forall (Φ).
+  wp_call. wp_apply (wp_try_select_blocking with "[-]").
+  - iSplit; first iFrame.
+    wp_auto. iApply "IH". iFrame.
+  - iModIntro. iIntros "% HΦ". wp_auto. iFrame.
+Qed.
+
+Local Lemma wp_try_select_case_nonblocking cs Ψ :
+  ∀ Φ,
+  (match cs with
+   | select_send_f t send_val send_chan send_handler =>
+       ∃ V γ (v : V) `(!IntoVal V) `(!chanG Σ V) `(!IntoValTyped V t),
+     ⌜ send_val = #v ⌝ ∗
+     is_channel (V:=V) (t:=t) send_chan γ ∗
+     send_au_fast send_chan v γ (WP #send_handler #() {{ Ψ }}) True
+  | select_receive_f t recv_chan recv_handler =>
+      ∃ V γ `(!IntoVal V) `(!IntoValTyped V t) `(!chanG Σ V),
+     is_channel (V:=V) (t:=t) recv_chan γ ∗
+     rcv_au_fast recv_chan γ (λ (v: V) ok,
+                                     WP #recv_handler (#v, #ok)%V {{ Ψ }}) True
+   end
+  ) ∧ (Φ (#(), #false)%V) -∗
+  (∀ retv, Ψ retv -∗ Φ (retv, #true)%V) -∗
+  WP chan.try_select_case #cs #false {{ Φ }}.
+Proof.
+  iIntros (Φ) "HΦ Hwand".
+  wp_call. rewrite [in (_ op)]to_val_unseal /=. destruct cs; wp_auto.
+  - repeat setoid_rewrite bi.and_exist_r.
+    iNamed "HΦ". iAssert (⌜ v = #a1 ⌝ ∗ is_channel ch a0)%I with "[-]" as "[-> #?]".
+    { iLeft in "HΦ". iDestruct "HΦ" as "(-> & #? & Hau)". iFrame "#". done. }
+    wp_apply (wp_TrySend with "[$]").
+    iLeft. iSplit.
+    + iLeft in "HΦ". iDestruct "HΦ" as "(_ & _ & Hau)".
+      iLeft in "Hau". iMod "Hau". iModIntro. iNext. iNamed "Hau".
+      iFrame. destruct s.
+      * iIntros "H". iSpecialize ("Hcont" with "[$]").
+        iMod "Hcont". iModIntro. wp_auto.
+        wp_apply (wp_wand with "Hcont").
+        iIntros (?) "HΦ". wp_auto. iApply "Hwand". iFrame.
+      * done.
+      * done.
+      * iIntros "H". iSpecialize ("Hcont" with "[$]"). iMod "Hcont". iModIntro.
+        wp_auto. wp_apply (wp_wand with "Hcont"). iIntros "% HΨ". wp_auto.
+        iApply "Hwand". done.
+      * done.
+      * done.
+      * done.
+    + wp_auto. iRight in "HΦ". done.
+  - repeat setoid_rewrite bi.and_exist_r.
+    iNamed "HΦ". iAssert (is_channel ch a0)%I with "[-]" as "#?".
+    { iLeft in "HΦ". iDestruct "HΦ" as "(#? & Hau)". iFrame "#". }
+    wp_apply (chan_au_recv.wp_TryReceive_nonblocking with "[$]").
+    iSplit.
+    + iLeft in "HΦ". iDestruct "HΦ" as "[_ Hau]".
+      iLeft in "Hau". iMod "Hau". iModIntro. iNext.
+      iNamed "Hau". iFrame. destruct s.
+      * destruct buff.
+        -- iFrame.
+        -- iIntros "H". iSpecialize ("Hcont" with "[$]").
+           iMod "Hcont". iModIntro. wp_auto.
+           wp_apply (wp_wand with "Hcont").
+           iIntros (?) "HΦ". wp_auto. iApply "Hwand". iFrame.
+      * done.
+      * iIntros "H". iSpecialize ("Hcont" with "[$]"). iMod "Hcont". iModIntro.
+        wp_auto. wp_apply (wp_wand with "Hcont"). iIntros "% HΨ". wp_auto.
+        iApply "Hwand". done.
+      * done.
+      * done.
+      * done.
+      * destruct draining.
+        -- iIntros "H". iSpecialize ("Hcont" with "[$]").
+           iMod "Hcont". iModIntro. wp_auto. wp_apply (wp_wand with "Hcont").
+           iIntros (ret) "HΦ". wp_auto. iApply "Hwand". iFrame.
+        -- iIntros "H". iSpecialize ("Hcont" with "[$]").
+           iMod "Hcont". iModIntro. wp_auto. wp_apply (wp_wand with "Hcont").
+           iIntros (ret) "HΦ". wp_auto. iApply "Hwand". iFrame.
+    + wp_auto. iRight in "HΦ". iFrame.
+Qed.
+
+Local Lemma wp_try_select_nonblocking (cases : list op) :
+  ∀ Ψ Φ,
+  ([∧ list] case ∈ cases,
+     match case with
+     | select_send_f t send_val send_chan send_handler =>
+         ∃ V γ (v : V) `(!IntoVal V) `(!chanG Σ V) `(!IntoValTyped V t),
+     ⌜ send_val = #v ⌝ ∗
+     is_channel (V:=V) (t:=t) send_chan γ ∗
+     send_au_fast send_chan v γ (WP #send_handler #() {{ Ψ }}) True
+  | select_receive_f t recv_chan recv_handler =>
+      ∃ V γ `(!IntoVal V) `(!IntoValTyped V t) `(!chanG Σ V),
+     is_channel (V:=V) (t:=t) recv_chan γ ∗
+     rcv_au_fast recv_chan γ (λ (v: V) ok,
+                                    WP #recv_handler (#v, #ok)%V {{ Ψ }}) True
+   end
+  ) ∧ Φ (#(), #false)%V -∗
+  □(∀ retv, Ψ retv -∗ Φ (retv, #true)%V) -∗
+  WP chan.try_select #cases #false {{ Φ }}.
+Proof.
+  simpl. iIntros (Ψ Φ) "HΦ #Hwand".
+  iLöb as "IH" forall (cases).
   wp_call.
-Admitted.
+  destruct cases.
+  { wp_auto. iRight in "HΦ". iApply "HΦ". }
+  wp_auto.
+  wp_apply (wp_try_select_case_nonblocking _ Ψ with "[-Hwand] [Hwand]").
+  2:{ iIntros (?) "HΨ". wp_auto. iApply "Hwand". iFrame. }
+  iSplit.
+  { simpl. iLeft in "HΦ". iLeft in "HΦ". iFrame. }
+  wp_auto. wp_apply ("IH" with "[HΦ]"); try iFrame.
+  iSplit.
+  - iLeft in "HΦ". simpl. iRight in "HΦ". iFrame.
+  - iRight in "HΦ". done.
+Qed.
 
 Lemma wp_select_nonblocking (cases : list op) (def: func.t) :
   ∀ Φ,
@@ -145,20 +389,25 @@ Lemma wp_select_nonblocking (cases : list op) (def: func.t) :
          ∃ V γ (v : V) `(!IntoVal V) `(!chanG Σ V) `(!IntoValTyped V t),
              ⌜ send_val = #v ⌝ ∗
              is_channel (V:=V) (t:=t) send_chan γ ∗
-             send_au_fast send_chan v γ (WP #send_handler #() {{ Φ }})
+             send_au_fast send_chan v γ (WP #send_handler #() {{ Φ }}) True
      | select_receive_f t recv_chan recv_handler =>
-         ∃ γ V `(!IntoVal V) `(!IntoValTyped V t) `(!chanG Σ V),
+         ∃ V γ `(!IntoVal V) `(!IntoValTyped V t) `(!chanG Σ V),
              is_channel (V:=V) (t:=t) recv_chan γ ∗
              rcv_au_fast recv_chan γ (λ (v: V) ok,
-               WP #recv_handler #v {{ Φ }})
+               WP #recv_handler (#v, #ok)%V {{ Φ }}) True
      end
   ) ∧ WP #def #() {{ Φ }} -∗
   WP chan.select_nonblocking #cases #def {{ Φ }}.
 Proof.
   iIntros (Φ) "Hcases".
-  wp_call.
-Admitted.
+  iLöb as "IH" forall (Φ).
+  wp_call. wp_apply (wp_try_select_nonblocking with "[-]").
+  - iSplit.
+    + iLeft in "Hcases". iFrame.
+    + iRight in "Hcases". wp_auto. iFrame.
+  - iModIntro. iIntros "% HΦ". wp_auto. iFrame.
+Qed.
 
-End proof.
+End select_proof.
 
 End chan.
